src/Prog.v
@@ -1,19 +1,80 @@
-From Coq Require Import Lia.
-From Coq Require Import Strings.String.
-From Coq Require Import Lists.List. Import ListNotations.
-From Coq Require Import Init.Nat.
+From Stdlib Require Import Lists.List. Import ListNotations.
+From stdpp Require Import base.
+From MRC Require Import Options.
+From MRC Require Import Tactics.
+From MRC Require Import Model.
+From MRC Require Import Stdppp.
 From MRC Require Import PredCalc.
 
-Inductive prog : Type :=
-  | PAsgn (x : string) (e : term)
+Section prog.
+  Context {M : model}.
+  Local Notation term := (term (value M)).
+  Local Notation formula := (formula (value M)).
+
+  Record ni_formula := mkNiFormula {
+    ni_formula_formula : formula;
+    ni_formula_no_initials : ∀ x, x ∈ formula_fvars ni_formula_formula → var_is_initial x = false
+  }.
+
+  Global Coercion ni_formula_formula : ni_formula >-> formula.
+
+  Inductive prog : Type :=
+  | PAsgn (x : variable) (t : term)
   | PSeq (p1 p2 : prog)
   | PIf (gcs : list gcom)
   | PDo (gcs : list gcom)
-  | PSpec (w : list string) (pre post : formula)
-  | PVar (x : string) (p : prog)
-  | PConst (x : string) (p : prog)
-with gcom :=
+  | PSpec (w : list variable) (pre : ni_formula) (post : formula)
+  | PVar (x : variable) (p : prog)
+  | PConst (x : variable) (p : prog)
+  with gcom :=
   | GCom (g : formula) (p : prog).
+
+  Definition gcom_guard (c : gcom) :=
+    match c with
+    | GCom a _ => a
+    end.
+
+  Definition gcom_cmd (c : gcom) :=
+    match c with
+    | GCom _ p => p
+    end.
+
+  Fixpoint gcoms_any_guard (gcoms : list gcom) : formula :=
+    match gcoms with
+    | [] => <! true !>
+    | h::t => <! `gcom_guard h` ∨ `gcoms_any_guard t` !>
+    end.
+
+  Fixpoint gcoms_all_cmds (gcoms : list gcom) (a : formula) : formula :=
+    match gcoms with
+    | [] => <! true !>
+    | h::t => <! (`gcom_guard h` => a) ∧ `gcoms_all_cmds t a` !>
+    end.
+
+  Fixpoint spec_post_wp (w : list variable) post A : formula :=
+    match w with
+    | [] => <! post => A !>
+    | h :: t => <! forall h, `spec_post_wp t post A` !>
+    end.
+
+  Fixpoint subst_initials A (w : list variable) : formula :=
+    match w with
+    | [] => A
+    | x :: xs => subst_initials (A[x \ (var_non_initial x)]) xs
+    end.
+
+  Fixpoint wp (p : prog) (A : formula) : formula :=
+    match p with
+    | PAsgn x e => A[x \ e]
+    | PSeq p1 p2 => wp p1 (wp p2 A)
+    | PIf gcs => <! `gcoms_any_guard (gcs)` ∧ `gcoms_all_cmds (gcs) A` !>
+    | PDo gcs => <! false !>
+    | PSpec w pre post => <! pre ∧ `subst_initials (spec_post_wp w post A) w` !>
+    | PVar x p => <! forall x, `wp p A` !>
+    | PConst x p => <! exists x, `wp p A` !>
+    end.
+
+End prog.
 
 Declare Custom Entry prog.
 Declare Custom Entry gcom.
@@ -27,105 +88,48 @@ Notation "e" := e (in custom prog_aux at level 0, e custom prog) : prog_scope.
 
 Notation "( x )" := x (in custom prog, x at level 99) : prog_scope.
 Notation "'`' x '`'" := (x)
-                  (in custom prog at level 0, only parsing,
-                  x constr at level 0) : prog_scope.
+                          (in custom prog at level 0, only parsing,
+                              x constr at level 0) : prog_scope.
 Notation "x" := x (in custom prog at level 0, x constr at level 0) : prog_scope.
 
-Notation "x := e" := (PAsgn x e) 
-  (in custom prog at level 95,  x constr at level 0,
-    e custom formula at level 85, no associativity) : prog_scope.
+Notation "x := e" := (PAsgn x e)
+                       (in custom prog at level 95,  x constr at level 0,
+                           e custom formula at level 85, no associativity) : prog_scope.
 
-Notation "x ; y" := (PSeq x y) 
-  (in custom prog at level 95, right associativity) : prog_scope.
+Notation "x ; y" := (PSeq x y)
+                      (in custom prog at level 95, right associativity) : prog_scope.
 
 Notation "x -> y" := (GCom x y)
-  (in custom gcom at level 60, x custom formula,
-    y custom prog,
-    no associativity) : prog_scope.
+                       (in custom gcom at level 60, x custom formula,
+                           y custom prog,
+                           no associativity) : prog_scope.
 
 Notation "'if' | x | .. | y 'fi'" :=
   (PIf (cons (x) .. (cons (y) nil) ..))
-  (in custom prog at level 95, 
-    x custom gcom, 
-    y custom gcom, no associativity) : prog_scope.
+    (in custom prog at level 95,
+        x custom gcom,
+        y custom gcom, no associativity) : prog_scope.
 
 Notation "'do' | x | .. | y 'od'" :=
   (PDo (cons (x) .. (cons (y) nil) ..))
-  (in custom prog at level 95, 
-    x custom gcom, 
-    y custom gcom, no associativity) : prog_scope.    
+    (in custom prog at level 95,
+        x custom gcom,
+        y custom gcom, no associativity) : prog_scope.
 
-Notation "x , .. , y : [ p , q ]" := 
+Notation "x , .. , y : [ p , q ]" :=
   (PSpec (cons x .. (cons y nil) ..) p q)
-  (in custom prog at level 95, no associativity,
-    x constr at level 0, y constr at level 0,
-    p custom formula at level 85, q custom formula at level 85) : prog_scope.
+    (in custom prog at level 95, no associativity,
+        x constr at level 0, y constr at level 0,
+        p custom formula at level 85, q custom formula at level 85) : prog_scope.
 
-Notation "'|[' 'var' x ',' y ']|' " := 
+Notation "'|[' 'var' x ',' y ']|' " :=
   (PVar x y)
-  (in custom prog at level 95, no associativity,
-    x constr at level 0, y custom prog) : prog_scope.    
+    (in custom prog at level 95, no associativity,
+        x constr at level 0, y custom prog) : prog_scope.
 
-Notation "'|[' 'const' x ',' y ']|' " := 
+Notation "'|[' 'const' x ',' y ']|' " :=
   (PConst x y)
-  (in custom prog at level 95, no associativity,
-    x constr at level 0, y custom prog at next level) : prog_scope.        
+    (in custom prog at level 95, no associativity,
+        x constr at level 0, y custom prog at next level) : prog_scope.
 
 Open Scope prog_scope.
-
-Definition gcom_guard (c : gcom) :=
-  match c with
-  | GCom a _ => a
-  end.
-
-Definition gcom_cmd (c : gcom) :=
-  match c with
-  | GCom _ p => p
-  end.  
-
-Fixpoint gcoms_any_guard (gcoms : list gcom) : formula :=
-  match gcoms with 
-  | [] => <[ true ]>
-  | h::t => <[ `gcom_guard h` \/ `gcoms_any_guard t` ]>
-  end.
-
-Fixpoint gcoms_all_cmds (gcoms : list gcom) (a : formula) : formula :=
-  match gcoms with
-  | [] => <[ true ]>
-  | h::t => <[ (`gcom_guard h` => a) /\ `gcoms_all_cmds t a` ]>
-  end.
-
-Fixpoint spec_post_wp (w : list string) post A :=
-  match w with
-  | [] => <[ post => A ]>
-  | h :: t => <[ forall h, `spec_post_wp t post A` ]>
-  end.
-
-Definition initsym x :=
-  append x "_0"%string.
-
-Definition is_initsym x := 
-  let l := String.length x in
-  if 3 <? l
-    then String.eqb (substring (l - 2) 2 x) "_0"
-    else false.
-  
-
-Fixpoint subst_initials f (w : list string) :=
-  match w with
-  | [] => f
-  | h :: t =>
-    let h0 := initsym h in
-    <[ (`subst_initials f t`)[h0 \ h] ]>
-  end.
-
-Fixpoint wp (p : prog) (A : formula) : formula :=
-  match p with
-  | PAsgn x e => A[x \ e]
-  | PSeq p1 p2 => wp p1 (wp p2 A)
-  | PIf gcs => <[ `gcoms_any_guard (gcs)` /\ `gcoms_all_cmds (gcs) A` ]>
-  | PDo gcs => <[ false ]>
-  | PSpec w pre post => <[ pre /\ `subst_initials (spec_post_wp w post A) w` ]>
-  | PVar x p => <[ forall x, `wp p A` ]>
-  | PConst x p => <[ exists x, `wp p A` ]>
-  end.
