src/PredCalcTactics.v
@@ -1,0 +1,457 @@
+From Equations Require Import Equations.
+From stdpp Require Import fin_maps.
+From MRC Require Import Options.
+From MRC Require Import Tactics.
+From MRC Require Import Model.
+From MRC Require Import Stdppp.
+From MRC Require Import PredCalcBasic PredCalcEquiv PredCalcSubst PredCalcFacts.
+From MRC Require Import PredCalcEquivLemmas.
+
+Ltac f_simpl :=
+  repeat match goal with
+    | H : context[<! ?A ∧ ?A !>] |- _ =>
+        rewrite f_and_idemp in H
+    | |- context[<! ?A ∧ ?A !>] =>
+        rewrite f_and_idemp
+
+    | H : context[<! ?A ∨ ?A !>] |- _ =>
+        rewrite f_or_idemp in H
+    | |- context[<! ?A ∨ ?A !>] =>
+        rewrite f_or_idemp
+
+    (*  f_and_absorb *)
+    | H : context[<! ?A ∧ (?A ∨ ?B) !>] |- _ =>
+        rewrite f_and_absorb in H
+    | H : context[<! (?A ∨ ?B) ∧ ?A !>] |- _ =>
+        let Heq := fresh "Heq" in
+        assert (<! (A ∨ B) ∧ A !> ≡ <! (A ∧ (A ∨ B)) !>) as Heq
+          by (rewrite f_and_comm; reflexivity);
+        rewrite Heq in H; rewrite f_and_absorb in H; clear Heq
+    | H : context[<! (?B ∨ ?A) ∧ ?A !>] |- _ =>
+        let Heq := fresh "Heq" in
+        assert (<! (B ∨ A) ∧ A !> ≡ <! (A ∧ (A ∨ B)) !>) as Heq
+          by (rewrite f_or_comm; rewrite f_and_comm; reflexivity);
+        rewrite Heq in H; rewrite f_and_absorb in H; clear Heq
+    | |- context[<! ?A ∧ (?A ∨ ?B) !>] =>
+        rewrite f_and_absorb
+    | |- context[<! (?A ∨ ?B) ∧ ?A !>] =>
+        let Heq := fresh "Heq" in
+        assert (<! (A ∨ B) ∧ A !> ≡ <! (A ∧ (A ∨ B)) !>) as Heq
+          by (rewrite f_and_comm; reflexivity);
+        rewrite Heq; rewrite f_and_absorb; clear Heq
+    | |- context[<! (?B ∨ ?A) ∧ ?A !>] =>
+        let Heq := fresh "Heq" in
+        assert (<! (B ∨ A) ∧ A !> ≡ <! (A ∧ (A ∨ B)) !>) as Heq
+          by (rewrite f_or_comm; rewrite f_and_comm; reflexivity);
+        rewrite Heq; rewrite f_and_absorb; clear Heq
+
+    (*  f_or_absorb *)
+    | H : context[<! ?A ∨ (?A ∧ ?B) !>] |- _ =>
+        rewrite f_or_absorb in H
+    | H : context[<! (?A ∧ ?B) ∨ ?A !>] |- _ =>
+        let Heq := fresh "Heq" in
+        assert (<! (A ∧ B) ∨ A !> ≡ <! (A ∨ (A ∧ B)) !>) as Heq
+          by (rewrite f_or_comm; reflexivity);
+        rewrite Heq in H; rewrite f_or_absorb in H; clear Heq
+    | H : context[<! (?B ∧ ?A) ∨ ?A !>] |- _ =>
+        let Heq := fresh "Heq" in
+        assert (<! (B ∧ A) ∨ A !> ≡ <! (A ∨ (A ∧ B)) !>) as Heq
+          by (rewrite f_and_comm; rewrite f_or_comm; reflexivity);
+        rewrite Heq in H; rewrite f_or_absorb in H; clear Heq
+    | |- context[<! ?A ∨ (?A ∧ ?B) !>] =>
+        rewrite f_or_absorb
+    | |- context[<! (?A ∧ ?B) ∨ ?A !>] =>
+        let Heq := fresh "Heq" in
+        assert (<! (A ∧ B) ∨ A !> ≡ <! (A ∨ (A ∧ B)) !>) as Heq
+          by (rewrite f_or_comm; reflexivity);
+        rewrite Heq; rewrite f_or_absorb; clear Heq
+    | |- context[<! (?B ∧ ?A) ∨ ?A !>] =>
+        let Heq := fresh "Heq" in
+        assert (<! (B ∧ A) ∨ A !> ≡ <! (A ∨ (A ∧ B)) !>) as Heq
+          by (rewrite f_and_comm; rewrite f_or_comm; reflexivity);
+        rewrite Heq; rewrite f_or_absorb; clear Heq
+
+    (* f_and_true *)
+    | H : context[FAnd ?A (FSimple AT_True)] |- _ =>
+        rewrite f_and_true in H
+    | H : context[FAnd (FSimple AT_True) ?A] |- _ =>
+        rewrite (f_and_comm <! true !> A) in H; rewrite f_and_true in H
+    | |- context[FAnd ?A (FSimple AT_True)] =>
+        rewrite f_and_true
+    | |- context[FAnd (FSimple AT_True) ?A] =>
+        rewrite (f_and_comm <! true !> A); rewrite f_and_true
+
+    (* f_and_false *)
+    | H : context[FAnd ?A (FSimple AT_False)] |- _ =>
+        rewrite f_and_false in H
+    | H : context[FAnd (FSimple AT_False) ?A] |- _ =>
+        rewrite (f_and_comm <! false !> A) in H; rewrite f_and_false in H
+    | |- context[FAnd ?A (FSimple AT_False)] =>
+        rewrite f_and_false
+    | |- context[FAnd (FSimple AT_False) ?A] =>
+        rewrite (f_and_comm <! false !> A); rewrite f_and_false
+
+    (* f_or_true *)
+    | H : context[FOr ?A (FSimple AT_True)] |- _ =>
+        rewrite f_or_true in H
+    | H : context[FOr (FSimple AT_True) ?A] |- _ =>
+        rewrite (f_or_comm <! true !> A) in H; rewrite f_or_true in H
+    | |- context[FOr ?A (FSimple AT_True)] =>
+        rewrite f_or_true
+    | |- context[FOr (FSimple AT_True) ?A] =>
+        rewrite (f_or_comm <! true !> A); rewrite f_or_true
+
+    (* f_or_false *)
+    | H : context[FOr ?A (FSimple AT_False)] |- _ =>
+        rewrite f_or_false in H
+    | H : context[FOr (FSimple AT_False) ?A] |- _ =>
+        rewrite (f_or_comm <! false !> A) in H; rewrite f_or_false in H
+    | |- context[FOr ?A (FSimple AT_False)] =>
+        rewrite f_or_false
+    | |- context[FOr (FSimple AT_False) ?A] =>
+        rewrite (f_or_comm <! false !> A); rewrite f_or_false
+
+    (* f_not_true *)
+    | H : context[FNot (FSimple AT_True)] |- _ =>
+        rewrite f_not_true in H
+    | |- context[FNot (FSimple AT_True)] =>
+        rewrite f_not_true
+
+    (* f_false_true *)
+    | H : context[FNot (FSimple AT_False)] |- _ =>
+        rewrite f_not_false in H
+    | |- context[FNot (FSimple AT_False)] =>
+        rewrite f_not_false
+
+    (* f_and_not_self *)
+    | H : context[<! ?A ∧ ¬ ?A !>] |- _ =>
+        rewrite f_and_not_self in H
+    | H : context[<! ¬ ?A ∧ ?A !>] |- _ =>
+        rewrite (f_and_comm (<! ¬ A !>) A) in H; rewrite f_and_not_self in H
+    | |- context[<! ?A ∧ ¬ ?A !>] =>
+        rewrite f_and_not_self
+    | |- context[<! ¬ ?A ∧ ?A !>] =>
+        rewrite (f_and_comm (<! ¬ A !>) A); rewrite f_and_not_self
+
+    (* f_excluded_middle *)
+    | H : context[<! ?A ∨ ¬ ?A !>] |- _ =>
+        rewrite f_excluded_middle in H
+    | H : context[<! ¬ ?A ∨ ?A !>] |- _ =>
+        rewrite (f_or_comm (<! ¬ A !>) A) in H; rewrite f_excluded_middle in H
+    | |- context[<! ?A ∨ ¬ ?A !>] =>
+        rewrite f_excluded_middle
+    | |- context[<! ¬ ?A ∨ ?A !>] =>
+        rewrite (f_or_comm (<! ¬ A !>) A); rewrite f_excluded_middle
+
+    (* f_not_stable *)
+    | H : context[<! ¬ ¬ ?A !>] |- _ =>
+        rewrite f_not_stable in H
+    | |- context[<! ¬ ¬ ?A !>] =>
+        rewrite f_not_stable
+
+    (* f_not_and *)
+    | H : context[<! ¬ (?A ∧ ?B) !>] |- _ =>
+        rewrite f_not_and in H
+    | |- context[<! ¬ (?A ∧ ?B) !>] =>
+        rewrite f_not_and
+
+    (* f_not_or *)
+    | H : context[<! ¬ (?A ∨ ?B) !>] |- _ =>
+        rewrite f_not_or in H
+    | |- context[<! ¬ (?A ∨ ?B) !>] =>
+        rewrite f_not_or
+
+    (* (* f_and_or_distr *) *)
+    (* | H : context[<! ?A ∧ (?B ∨ ?C) !>] |- _ => *)
+    (*     rewrite f_and_or_distr in H *)
+    (* | H : context[<! (?B ∨ ?C) ∧ ?A !>] |- _ => *)
+    (*     rewrite (f_and_comm (?B ∨ ?C) ?A) in H; rewrite f_and_or_distr in H *)
+    (* | |- context[<! ?A ∧ (?B ∨ ?C) !>] => *)
+    (*     rewrite f_and_or_distr *)
+    (* | |- context[<! (?B ∨ ?C) ∧ ?A !>] => *)
+    (*     rewrite (f_and_comm (?B ∨ ?C) ?A); rewrite f_and_or_distr *)
+
+    (* (* f_or_and_distr *) *)
+    (* | H : context[<! ?A ∨ (?B ∧ ?C) !>] |- _ => *)
+    (*     rewrite f_or_and_distr in H *)
+    (* | H : context[<! (?B ∧ ?C) ∨ ?A !>] |- _ => *)
+    (*     rewrite (f_or_comm (?B ∧ ?C) ?A) in H; rewrite f_or_and_distr in H *)
+    (* | |- context[<! ?A ∨ (?B ∧ ?C) !>] => *)
+    (*     rewrite f_or_and_distr *)
+    (* | |- context[<! (?B ∨ ?C) ∧ ?A !>] => *)
+    (*     rewrite (f_and_comm (?B ∨ ?C) ?A); rewrite f_or_and_distr *)
+
+    (*  f_and_not_absorb *)
+    | H : context[<! ?A ∧ (¬ ?A ∨ ?B) !>] |- _ =>
+        rewrite f_and_not_absorb in H
+    | H : context[<! (¬ ?A ∨ ?B) ∧ ?A !>] |- _ =>
+        let Heq := fresh "Heq" in
+        assert (<! (¬ A ∨ B) ∧ A !> ≡ <! (A ∧ (¬ A ∨ B)) !>) as Heq
+          by (rewrite f_and_comm; reflexivity);
+        rewrite Heq in H; rewrite f_and_not_absorb in H; clear Heq
+    | H : context[<! (?B ∨ ¬ ?A) ∧ ?A !>] |- _ =>
+        let Heq := fresh "Heq" in
+        assert (<! (B ∨ ¬ A) ∧ A !> ≡ <! (A ∧ (¬ A ∨ B)) !>) as Heq
+          by (rewrite f_or_comm; rewrite f_and_comm; reflexivity);
+        rewrite Heq in H; rewrite f_and_not_absorb in H; clear Heq
+    | |- context[<! ?A ∧ (¬ ?A ∨ ?B) !>] =>
+        rewrite f_and_not_absorb
+    | |- context[<! (¬ ?A ∨ ?B) ∧ ?A !>] =>
+        let Heq := fresh "Heq" in
+        assert (<! (¬ A ∨ B) ∧ A !> ≡ <! (A ∧ (¬ A ∨ B)) !>) as Heq
+          by (rewrite f_and_comm; reflexivity);
+        rewrite Heq; rewrite f_and_not_absorb; clear Heq
+    | |- context[<! (?B ∨ ¬ ?A) ∧ ?A !>] =>
+        let Heq := fresh "Heq" in
+        assert (<! (B ∨ ¬ A) ∧ A !> ≡ <! (A ∧ (¬ A ∨ B)) !>) as Heq
+          by (rewrite f_or_comm; rewrite f_and_comm; reflexivity);
+        rewrite Heq; rewrite f_and_not_absorb; clear Heq
+
+    (*  f_or_not_absorb *)
+    | H : context[<! ?A ∨ (¬ ?A ∧ ?B) !>] |- _ =>
+        rewrite f_or_not_absorb in H
+    | H : context[<! (¬ ?A ∧ ?B) ∨ ?A !>] |- _ =>
+        let Heq := fresh "Heq" in
+        assert (<! (¬ A ∧ B) ∨ A !> ≡ <! (A ∨ (¬ A ∧ B)) !>) as Heq
+          by (rewrite f_or_comm; reflexivity);
+        rewrite Heq in H; rewrite f_or_not_absorb in H; clear Heq
+    | H : context[<! (?B ∧ ¬ ?A) ∨ ?A !>] |- _ =>
+        let Heq := fresh "Heq" in
+        assert (<! (B ∧ ¬ A) ∨ A !> ≡ <! (A ∨ (¬ A ∧ B)) !>) as Heq
+          by (rewrite f_and_comm; rewrite f_or_comm; reflexivity);
+        rewrite Heq in H; rewrite f_or_not_absorb in H; clear Heq
+    | |- context[<! ?A ∨ (¬ ?A ∧ ?B) !>] =>
+        rewrite f_or_not_absorb
+    | |- context[<! (¬ ?A ∧ ?B) ∨ ?A !>] =>
+        let Heq := fresh "Heq" in
+        assert (<! (¬ A ∧ B) ∨ A !> ≡ <! (A ∨ (¬ A ∧ B)) !>) as Heq
+          by (rewrite f_or_comm; reflexivity);
+        rewrite Heq; rewrite f_or_not_absorb; clear Heq
+    | |- context[<! (?B ∧ ¬ ?A) ∨ ?A !>] =>
+        let Heq := fresh "Heq" in
+        assert (<! (B ∧ ¬ A) ∨ A !> ≡ <! (A ∨ (¬ A ∧ B)) !>) as Heq
+          by (rewrite f_and_comm; rewrite f_or_comm; reflexivity);
+        rewrite Heq; rewrite f_or_not_absorb; clear Heq
+
+    (* f_implies_self *)
+    | H : context[<! ?A => ?A !>] |- _ =>
+        rewrite f_implies_self in H
+    | |- context[<! ?A => ?A !>] =>
+        rewrite f_implies_self
+
+    (* f_not_impl *)
+    | H : context[<! ¬ (?A => ?B) !>] |- _ =>
+        rewrite f_not_impl in H
+    | |- context[<! ¬ (?A => ?B) !>] =>
+        rewrite f_not_impl
+
+    (* f_implies_true *)
+    | H : context[<! ?A => true !>] |- _ =>
+        rewrite f_implies_true in H
+    | |- context[<! ?A => true !>] =>
+        rewrite f_implies_true
+
+    (* f_true_implies *)
+    | H : context[<! true => ?A !>] |- _ =>
+        rewrite f_true_implies in H
+    | |- context[<! true => ?A !>] =>
+        rewrite f_true_implies
+
+    (* f_implies_false *)
+    | H : context[<! ?A => false !>] |- _ =>
+        rewrite f_implies_false in H
+    | |- context[<! ?A => false !>] =>
+        rewrite f_implies_false
+
+    (* f_false_implies *)
+    | H : context[<! false => ?A !>] |- _ =>
+        rewrite f_false_implies in H
+    | |- context[<! false => ?A !>] =>
+        rewrite f_false_implies
+
+    (* f_implies_not_self *)
+    | H : context[<! ?A => ¬ ?A !>] |- _ =>
+        rewrite f_implies_not_self in H
+    | |- context[<! ?A => ¬ ?A !>] =>
+        rewrite f_implies_not_self
+
+    (* f_not_implies_self *)
+    | H : context[<! ¬ ?A => ?A !>] |- _ =>
+        rewrite f_not_implies_self in H
+    | |- context[<! ¬ ?A => ?A !>] =>
+        rewrite f_not_implies_self
+
+    (* f_iff_equiv3 *)
+    | H : context[<! ¬ ?A <=> ¬ ?B !>] |- _ =>
+        rewrite <- f_iff_negate in H
+    | |- context[<! ¬ ?A <=> ¬ ?B !>] =>
+        rewrite <- f_iff_negate
+
+    (* f_iff_self *)
+    | H : context[<! ?A <=> ?A !>] |- _ =>
+        rewrite f_iff_self in H
+    | |- context[<! ?A <=> ?A !>] =>
+        rewrite f_iff_self
+
+    (* f_iff_not_self *)
+    | H : context[<! ?A <=> ¬ ?A !>] |- _ =>
+        rewrite f_iff_not_self in H
+    | H : context[<! ¬ ?A <=> ?A !>] |- _ =>
+        rewrite (f_iff_comm (<! ¬ A !>) A) in H; rewrite f_iff_not_self in H
+    | |- context[<! ?A <=> ?A !>] =>
+        rewrite f_iff_self
+    | |- context[<! ¬ ?A <=> ?A !>] =>
+        rewrite (f_iff_comm (<! ¬ A !>) A); rewrite f_iff_not_self
+
+    (* f_iff_true *)
+    | H : context[FIff ?A (FSimple AT_True)] |- _ =>
+        rewrite f_iff_true in H
+    | H : context[FIff (FSimple AT_True) ?A] |- _ =>
+        rewrite (f_iff_comm (<! true !>) A) in H; rewrite f_iff_true in H
+    | |- context[FIff ?A (FSimple AT_True)] =>
+        rewrite f_iff_true
+    | |- context[FIff (FSimple AT_True) ?A] =>
+        rewrite (f_iff_comm (<! true !>) A); rewrite f_iff_true
+
+    (* f_iff_false *)
+    | H : context[FIff ?A (FSimple AT_False)] |- _ =>
+        rewrite f_iff_false in H
+    | H : context[FIff (FSimple AT_False) ?A] |- _ =>
+        rewrite (f_iff_comm (<! false !>) A) in H; rewrite f_iff_false in H
+    | |- context[FIff ?A (FSimple AT_False)] =>
+        rewrite f_iff_false
+    | |- context[FIff (FSimple AT_False) ?A] =>
+        rewrite (f_iff_comm (<! false !>) A); rewrite f_iff_false
+
+    (*  f_iff_and_absorb *)
+    | H : context[<! ?A <=> (?A ∧ ?B) !>] |- _ =>
+        rewrite f_iff_and_absorb in H
+    | H : context[<! (?A ∧ ?B) <=> ?A !>] |- _ =>
+        let Heq := fresh "Heq" in
+        assert (<! (A ∧ B) <=> A !> ≡ <! (A <=> (A ∧ B)) !>) as Heq
+          by (rewrite f_iff_comm; reflexivity);
+        rewrite Heq in H; rewrite f_iff_and_absorb in H; clear Heq
+    | H : context[<! (?B ∧ ?A) <=> ?A !>] |- _ =>
+        let Heq := fresh "Heq" in
+        assert (<! (B ∧ A) <=> A !> ≡ <! (A <=> (A ∧ B)) !>) as Heq
+          by (rewrite f_and_comm; rewrite f_iff_comm; reflexivity);
+        rewrite Heq in H; rewrite f_iff_and_absorb in H; clear Heq
+    | |- context[<! ?A <=> (?A ∧ ?B) !>] =>
+        rewrite f_iff_and_absorb
+    | |- context[<! (?A ∧ ?B) <=> ?A !>] =>
+        let Heq := fresh "Heq" in
+        assert (<! (A ∧ B) <=> A !> ≡ <! (A <=> (A ∧ B)) !>) as Heq
+          by (rewrite f_iff_comm; reflexivity);
+        rewrite Heq; rewrite f_iff_and_absorb; clear Heq
+    | |- context[<! (?B ∧ ?A) <=> ?A !>] =>
+        let Heq := fresh "Heq" in
+        assert (<! (B ∧ A) <=> A !> ≡ <! (A <=> (A ∧ B)) !>) as Heq
+          by (rewrite f_and_comm; rewrite f_iff_comm; reflexivity);
+        rewrite Heq; rewrite f_iff_and_absorb; clear Heq
+
+    (* f_not_forall *)
+    | H : context[<! ¬ forall ?x, ?A !>] |- _ =>
+        rewrite f_not_forall in H
+    | |- context[<! ¬ forall ?x, ?A !>] =>
+        rewrite f_not_forall
+
+    (* f_not_exists *)
+    | H : context[<! ¬ exists ?x, ?A !>] |- _ =>
+        rewrite f_not_exists in H
+    | |- context[<! ¬ exists ?x, ?A !>] =>
+        rewrite f_not_exists
+
+    (*  f_iff_or_absorb *)
+    | H : context[<! ?A <=> (?A ∨ ?B) !>] |- _ =>
+        rewrite f_iff_or_absorb in H
+    | H : context[<! (?A ∨ ?B) <=> ?A !>] |- _ =>
+        let Heq := fresh "Heq" in
+        assert (<! (A ∨ B) <=> A !> ≡ <! (A <=> (A ∨ B)) !>) as Heq
+          by (rewrite f_iff_comm; reflexivity);
+        rewrite Heq in H; rewrite f_iff_or_absorb in H; clear Heq
+    | H : context[<! (?B ∨ ?A) <=> ?A !>] |- _ =>
+        let Heq := fresh "Heq" in
+        assert (<! (B ∨ A) <=> A !> ≡ <! (A <=> (A ∨ B)) !>) as Heq
+          by (rewrite f_or_comm; rewrite f_iff_comm; reflexivity);
+        rewrite Heq in H; rewrite f_iff_or_absorb in H; clear Heq
+    | |- context[<! ?A <=> (?A ∨ ?B) !>] =>
+        rewrite f_iff_or_absorb
+    | |- context[<! (?A ∨ ?B) <=> ?A !>] =>
+        let Heq := fresh "Heq" in
+        assert (<! (A ∨ B) <=> A !> ≡ <! (A <=> (A ∨ B)) !>) as Heq
+          by (rewrite f_iff_comm; reflexivity);
+        rewrite Heq; rewrite f_iff_or_absorb; clear Heq
+    | |- context[<! (?B ∨ ?A) <=> ?A !>] =>
+        let Heq := fresh "Heq" in
+        assert (<! (B ∨ A) <=> A !> ≡ <! (A <=> (A ∨ B)) !>) as Heq
+          by (rewrite f_or_comm; rewrite f_iff_comm; reflexivity);
+        rewrite Heq; rewrite f_iff_or_absorb; clear Heq
+
+    (* automatically prove A ≡ A and discharge ¬ A ≡ A *)
+    | H : ¬ (<! ?A !> ≡ <! ?A !>) |- _ =>
+        specialize (H (reflexivity A)); destruct H
+    | |- <! ?A !> ≡ <! ?A !> =>
+        reflexivity
+
+    (* f_and_cancel_l and f_and_cancel_r *)
+    | |- <! ?A ∧ ?B !> ≡ <! ?A ∧ ?C !> =>
+        apply f_and_cancel_l
+    | |- <! ?B ∧ ?A !> ≡ <! ?A ∧ ?C !> =>
+        rewrite (f_and_comm B A); apply f_and_cancel_l
+    | |- <! ?A ∧ ?B !> ≡ <! ?C ∧ ?A !> =>
+        rewrite (f_and_comm C A); apply f_and_cancel_l
+    | |- <! ?B ∧ ?A !> ≡ <! ?C ∧ ?A !> =>
+        apply f_and_cancel_r
+
+    (* f_or_cancel_l and f_or_cancel_r *)
+    | |- <! ?A ∨ ?B !> ≡ <! ?A ∨ ?C !> =>
+        apply f_or_cancel_l
+    | |- <! ?B ∨ ?A !> ≡ <! ?A ∨ ?C !> =>
+        rewrite (f_or_comm B A); apply f_or_cancel_l
+    | |- <! ?A ∨ ?B !> ≡ <! ?C ∨ ?A !> =>
+        rewrite (f_or_comm C A); apply f_or_cancel_l
+    | |- <! ?B ∨ ?A !> ≡ <! ?C ∨ ?A !> =>
+        apply f_or_cancel_r
+
+    (* f_impl_cancel_l and f_impl_cancel_r *)
+    | |- <! ?A => ?B !> ≡ <! ?A => ?C !> =>
+        apply f_impl_cancel_l
+    | |- <! ?B => ?A !> ≡ <! ?C => ?A !> =>
+        apply f_impl_cancel_r
+
+    (* f_subst_cancel *)
+    | |- <! ?A [ ?x \ ?t ]!> ≡ <! ?B [ ?x \ ?t ] !> =>
+        apply f_subst_cancel
+    | |- <! ?A [ ?x \ ?t1 ]!> ≡ <! ?A [ ?x \ ?t2 ] !> =>
+        apply f_subst_cancel_term
+
+    (* f_ent_and_cancel_l and f_ent_and_cancel_r *)
+    | |- <! ?A ∧ ?B !> ⇛ <! ?A ∧ ?C !> =>
+        apply f_ent_and_cancel_l
+    | |- <! ?B ∧ ?A !> ⇛ <! ?A ∧ ?C !> =>
+        rewrite (f_and_comm B A); apply f_ent_and_cancel_l
+    | |- <! ?A ∧ ?B !> ⇛ <! ?C ∧ ?A !> =>
+        rewrite (f_and_comm C A); apply f_ent_and_cancel_l
+    | |- <! ?B ∧ ?A !> ⇛ <! ?C ∧ ?A !> =>
+        apply f_ent_and_cancel_r
+
+    (* f_ent_or_cancel_l and f_ent_or_cancel_r *)
+    | |- <! ?A ∨ ?B !> ⇛ <! ?A ∨ ?C !> =>
+        apply f_ent_or_cancel_l
+    | |- <! ?B ∨ ?A !> ⇛ <! ?A ∨ ?C !> =>
+        rewrite (f_or_comm B A); apply f_ent_or_cancel_l
+    | |- <! ?A ∨ ?B !> ⇛ <! ?C ∨ ?A !> =>
+        rewrite (f_or_comm C A); apply f_ent_or_cancel_l
+    | |- <! ?B ∨ ?A !> ⇛ <! ?C ∨ ?A !> =>
+        apply f_ent_or_cancel_r
+
+    (* f_ent_impl_cancel_l and f_ent_impl_cancel_r *)
+    | |- <! ?A => ?B !> ⇛ <! ?A => ?C !> =>
+        apply f_ent_impl_cancel_l
+    | |- <! ?B => ?A !> ⇛ <! ?C => ?A !> =>
+        apply f_ent_impl_cancel_r
+
+    (* f_ent_subst_cancel *)
+    | |- <! ?A [ ?x \ ?t ]!> ⇛ <! ?B [ ?x \ ?t ] !> =>
+        apply f_ent_subst_cancel
+  end.
