src/Refinement.v
@@ -1,48 +1,75 @@
-From Coq Require Import Lia.
-From Coq Require Import Strings.String.
-From Coq Require Import Lists.List. Import ListNotations.
+From Stdlib Require Import Lists.List. Import ListNotations.
+From stdpp Require Import base tactics listset.
+From MRC Require Import Options.
+From MRC Require Import Tactics.
+From MRC Require Import Model.
+From MRC Require Import Stdppp.
 From MRC Require Import PredCalc.
-From MRC Require Import FormulaProps.
 From MRC Require Import Prog.
 
-Open Scope general_fassertion_scope.
-Definition refines (p1 p2 : prog) fctx pctx :=
-  forall A,
-    (forall x, is_free_in (initsym x) A = false) ->
-    formula_implies (wp p1 A) (wp p2 A) fctx pctx.
+Section refinement.
+  Context {M : model}.
+  Local Notation prog := (@prog M).
+  Local Notation formula := (formula (value M)).
+  Local Notation ni_formula := (@ni_formula M).
 
-Declare Scope general_refinement_scope.
-Notation "x '[=' y" := (forall fctx pctx, refines x y fctx pctx) 
-    (in custom prog at level 60, 
-    x custom prog,
-    y custom prog at level 95,
-    only parsing)
-  : general_refinement_scope.
+  Implicit Types A B C : formula.
+  Implicit Types pre : ni_formula.
+  (* Implicit Types w : list variable. *)
 
-Notation "x '⊑' y" := (forall fctx pctx, refines x y fctx pctx) 
-    (in custom prog at level 60, 
-    x custom prog,
-    y custom prog at level 95,
-    only printing,
-    format "x  '⊑'  y")
-  : general_refinement_scope.  
+  Definition refines (p1 p2 : prog) :=
+    ∀ A,
+      (∀ x, x ∈ formula_fvars A → var_is_initial x = false) ->
+      wp p1 A ⇛ (wp p2 A).
 
-Open Scope general_refinement_scope.
+  Notation "x '⊑' y" := (refines x y)
+                          (in custom prog at level 60,
+                              x custom prog,
+                              y custom prog at level 95)
+      : mrc_scope.
 
-Theorem assignment : forall pre post w E,
-  pre ==> post[w \ E] ->
-  <{ w : [pre, post] [= w := E }>.
-  intros pre post w E H. unfold refines. intros fctx pctx A H0.
+  Lemma r_strengthen_post pre post post' w :
+    post' ⇛ post ->
+    <{ w : [pre, post] ⊑ w : [pre, post'] }>.
+  Proof.
+    intros Hent A Hinit. simpl. f_simpl. apply f_forall_ent. intros.
+    f_simpl. assumption.
+  Qed.
+
+  Lemma r_weaken_pre pre pre' post w :
+    pre ⇛ pre' ->
+    <{ w : [pre, post] ⊑ w : [pre', post] }>.
+  Proof.
+    intros Hent A Hinit. simpl. f_simpl. assumption.
+  Qed.
+
+  Lemma assignment : forall pre post x E,
+      pre ⇛ post[x \ E] ->
+      <{ x : [pre, post] ⊑ x := E }>.
+  Proof.
+    intros pre post w E H A Hfree. simpl.
+    assert ((ni_formula_formula pre) ≡ pre [w \ (var_non_initial w)]) by admit.
+    rewrite H0.
+    rewrite <- simpl_subst_and.
+    rewrite <- (f_forall_one_point).
+    2:{ admit. }
+    2: {  }
+    -
+      simpl.
+  Qed.
+
+
+
+
+
+Lemma assignment : forall pre post x E,
+  pre ⇛ post[x \ E] ->
+  <{ x : [pre, post] ⊑ x := E }>.
+Proof.
+  intros pre post w E H A Hfree. simpl. etrans.
+  -
   simpl. 
 Qed.
 
 Compute wp <{ x : [1 < 2, 2 < 3] }> <[ 5 = 7 ]>.
-
-Theorem strengthen_post : forall pre post post' w,
-  post' ==> post ->
-  <{ w : [pre, post] [= w : [pre, post'] }>.
-Proof.
-  intros pre post post' w H. unfold refines. intros fctx pctx A.
-  simpl.  
-
 
